\section{玻尔兹曼统计}


\mathrm{d}q \quad \text{vs} \quad \dj q\\


配分函数
\begin{equation}
    Z_1=\sum_l{\omega _l\mathrm{e}^{-\beta \varepsilon _l}}
\end{equation}
粒子数
\begin{equation}
    N=\mathrm{e}^{-\alpha}Z_1
\end{equation}
内能
\begin{equation}
    U=-N\frac{\partial}{\partial \beta}\ln Z_1
\end{equation}
广义力-压强
\begin{equation}
    Y=-\frac{N}{\beta}\frac{\partial}{\partial y}\ln Z_1\Rightarrow p=\frac{N}{\beta}\frac{\partial}{\partial V}\ln Z_1
    
\end{equation}
熵
\begin{equation}
    S=Nk\left( \ln Z_1-\beta \frac{\partial}{\partial \beta}\ln Z_1 \right) =k\ln \Omega 
\end{equation}

推导：

配分函数
\begin{equation}
    Z_1=\sum_l{\omega _l\mathrm{e}^{-\beta \varepsilon _l}}
\end{equation}
玻尔兹曼分布
\begin{equation}
    
\end{equation}


粒子数
\begin{equation}
    \begin{aligned}
        N&=\sum_l{a_l}
\\
&=\sum_l{\omega _l\mathrm{e}^{-\alpha -\beta \varepsilon _l}}
\\
&=\mathrm{e}^{-\alpha}\sum_l{\omega _l\mathrm{e}^{-\beta \varepsilon _l}}
\\
&=\mathrm{e}^{-\alpha}Z_1
    \end{aligned}
\end{equation}


内能
\begin{equation}
    \begin{aligned}
        U&=\sum_l{\varepsilon _la_l}
\\
&=\sum_l{\varepsilon _l\omega _l\mathrm{e}^{-\alpha -\beta \varepsilon _l}}
\\
&=\mathrm{e}^{-\alpha}\sum_l{\omega _l\left( \varepsilon _l\mathrm{e}^{-\beta \varepsilon _l} \right)}
\\
&=\mathrm{e}^{-\alpha}\sum_l{\omega _l\left( -\frac{\partial}{\partial \beta}\mathrm{e}^{-\beta \varepsilon _l} \right)}
\\
&=\mathrm{e}^{-\alpha}\left( -\frac{\partial}{\partial \beta}\sum_l{\omega _l\mathrm{e}^{-\beta \varepsilon _l}} \right) 
\\
&=\mathrm{e}^{-\alpha}\left( -\frac{\partial}{\partial \beta} \right) \sum_l{\omega _l\mathrm{e}^{-\beta \varepsilon _l}}
\\
&=-\mathrm{e}^{-\alpha}\frac{\partial}{\partial \beta}\sum_l{\omega _l\mathrm{e}^{-\beta \varepsilon _l}}
\\
&=-\frac{N}{Z_1}\frac{\partial}{\partial \beta}Z_1
\\
&=-N\frac{\partial}{\partial \beta}\ln Z_1
    \end{aligned}
\end{equation}



广义力
\begin{equation}
    \begin{aligned}
        Y&=\sum_l{\frac{\partial \varepsilon _l}{\partial y}a_l}
\\
&=\sum_l{\frac{\partial \varepsilon _l}{\partial y}\omega _l\mathrm{e}^{-\alpha -\beta \varepsilon _l}}
\\
&=\mathrm{e}^{-\alpha}\sum_l{\omega _l\left( \frac{\partial \varepsilon _l}{\partial y}\mathrm{e}^{-\beta \varepsilon _l} \right)}
\\
&=\mathrm{e}^{-\alpha}\sum_l{\omega _l\left( -\frac{1}{\beta}\frac{\partial}{\partial y}\mathrm{e}^{-\beta \varepsilon _l} \right)}
\\
&=\mathrm{e}^{-\alpha}\left( -\frac{1}{\beta}\frac{\partial}{\partial y}\sum_l{\omega _l\mathrm{e}^{-\beta \varepsilon _l}} \right) 
\\
&=\mathrm{e}^{-\alpha}\left( -\frac{1}{\beta}\frac{\partial}{\partial y} \right) \sum_l{\omega _l\mathrm{e}^{-\beta \varepsilon _l}}
\\
&=-\mathrm{e}^{-\alpha}\frac{1}{\beta}\frac{\partial}{\partial y}\sum_l{\omega _l\mathrm{e}^{-\beta \varepsilon _l}}
\\
&=-\frac{N}{Z_1}\frac{1}{\beta}\frac{\partial}{\partial y}Z_1
\\
&=-\frac{N}{\beta}\frac{1}{Z_1}\frac{\partial}{\partial y}Z_1
\\
&=-\frac{N}{\beta}\frac{\partial}{\partial y}\ln Z_1
    \end{aligned}
\end{equation}
压强，取$Y=-p,y=V$
\begin{equation}
    \begin{aligned}
        p=\frac{N}{\beta}\frac{\partial}{\partial V}\ln Z_1
    \end{aligned}
\end{equation}


\begin{equation}
    \begin{aligned}
        
    \end{aligned}
\end{equation}


\begin{equation}
    \begin{aligned}
        
    \end{aligned}
\end{equation}

