\section{系综理论}





































%%%%%%%%%%%%%%%%%%%%%%%%%%%%%%%%%%%%%%%%%%%%%%%%%%%%%%%%
\subsection{巨正则系综理论的热力学公式}



平均粒子数
\begin{equation}
    \begin{aligned}
        \bar{N}&=\sum_N{\sum_s{N\rho _{s,N}}}
\\
&=\sum_N{\sum_s{\frac{N}{\varXi}e^{-\alpha N-\beta E_s}}}
\\
&=\frac{1}{\varXi}\sum_N{\sum_s{Ne^{-\alpha N-\beta E_s}}}
\\
&=\frac{1}{\varXi}\sum_N{\sum_s{\left( -\frac{\partial}{\partial \alpha}e^{-\alpha N-\beta E_s} \right)}}
\\
&=\frac{1}{\varXi}\left( -\frac{\partial}{\partial \alpha}\sum_N{\sum_s{e^{-\alpha N-\beta E_s}}} \right) 
\\
&=\frac{1}{\varXi}\left( -\frac{\partial}{\partial \alpha} \right) \sum_N{\sum_s{e^{-\alpha N-\beta E_s}}}
\\
&=-\frac{1}{\varXi}\frac{\partial}{\partial \alpha}\sum_N{\sum_s{e^{-\alpha N-\beta E_s}}}
\\
&=-\frac{1}{\varXi}\frac{\partial}{\partial \alpha}\varXi 
\\
&=-\frac{\partial}{\partial \alpha}\ln \varXi 
    \end{aligned}
\end{equation}
内能
\begin{equation}
    \begin{aligned}
        U=\bar{E}&=\sum_N{\sum_s{E_s\rho _{s,N}}}
\\
&=\sum_N{\sum_s{\frac{E_s}{\varXi}e^{-\alpha N-\beta E_s}}}
\\
&=\frac{1}{\varXi}\sum_N{\sum_s{E_se^{-\alpha N-\beta E_s}}}
\\
&=\frac{1}{\varXi}\sum_N{\sum_s{\left( -\frac{\partial}{\partial \beta}e^{-\alpha N-\beta E_s} \right)}}
\\
&=\frac{1}{\varXi}\left( -\frac{\partial}{\partial \beta}\sum_N{\sum_s{e^{-\alpha N-\beta E_s}}} \right) 
\\
&=\frac{1}{\varXi}\left( -\frac{\partial}{\partial \beta} \right) \sum_N{\sum_s{e^{-\alpha N-\beta E_s}}}
\\
&=-\frac{1}{\varXi}\frac{\partial}{\partial \beta}\sum_N{\sum_s{e^{-\alpha N-\beta E_s}}}
\\
&=-\frac{1}{\varXi}\frac{\partial}{\partial \beta}\varXi 
\\
&=-\frac{\partial}{\partial \beta}\ln \varXi 
    \end{aligned}
\end{equation}
广义力
\begin{equation}
    \begin{aligned}
        Y&=\sum_N{\sum_s{\frac{\partial E_s}{\partial y}\rho _{s,N}}}
\\
&=\sum_N{\sum_s{\frac{\partial E_s}{\partial y}\frac{1}{\varXi}e^{-\alpha N-\beta E_s}}}
\\
&=\frac{1}{\varXi}\sum_N{\sum_s{\frac{\partial E_s}{\partial y}e^{-\alpha N-\beta E_s}}}
\\
&=\frac{1}{\varXi}\sum_N{\sum_s{\left( -\frac{1}{\beta}\frac{\partial}{\partial y}e^{-\alpha N-\beta E_s} \right)}}
\\
&=\frac{1}{\varXi}\left( -\frac{1}{\beta}\frac{\partial}{\partial y}\sum_N{\sum_s{e^{-\alpha N-\beta E_s}}} \right) 
\\
&=\frac{1}{\varXi}\left( -\frac{1}{\beta}\frac{\partial}{\partial y} \right) \sum_N{\sum_s{e^{-\alpha N-\beta E_s}}}
\\
&=-\frac{1}{\varXi}\frac{1}{\beta}\frac{\partial}{\partial y}\sum_N{\sum_s{e^{-\alpha N-\beta E_s}}}
\\
&=-\frac{1}{\beta}\frac{1}{\varXi}\frac{\partial}{\partial y}\varXi 
\\
&=-\frac{1}{\beta}\frac{\partial}{\partial y}\ln \varXi 
    \end{aligned}
\end{equation}


